proof/agp32_MEM_Data_CorrectScript.sml
@@ -1333,6 +1333,51 @@ Proof
 QED
 
 
+(** acc_res **)
+Theorem agp32_Rel_ag32_acc_res_correct:
+  !fext fbits a t I.
+    is_mem fext_accessor_circuit (agp32 fext fbits) fext ==>
+    is_sch I (agp32 fext fbits) a ==>
+    Rel I (fext t) (agp32 fext fbits (t-1)) (agp32 fext fbits t) a t ==>
+    I (5, SUC t) <> NONE ==>
+    (agp32 fext fbits (SUC t)).WB.WB_state_flag ==>
+    (agp32 fext fbits (SUC t)).WB.WB_opc = 8w ==>
+    (agp32 fext fbits (SUC t)).acc_res = acc_res (FUNPOW Next (THE (I (5,SUC t)) − 1) a)
+Proof
+  rw [] >> Cases_on `enable_stg 5 (agp32 fext fbits t)` >-
+   (`(agp32 fext fbits (SUC t)).state = 2w` by fs [agp32_state_acc_WB_enable] >>
+    gs [enable_stg_def,agp32_WB_state_flag_and_state]) >>
+  Q.ABBREV_TAC `s = agp32 fext fbits t` >>
+  Q.ABBREV_TAC `s' = procs [agp32_next_state; WB_pipeline; MEM_pipeline; EX_pipeline;
+                            REG_write; ID_pipeline; IF_PC_update] (fext t) s s` >>
+  `(agp32 fext fbits (SUC t)).acc_res = (Acc_compute (fext t) s s').acc_res`
+    by gs [agp32_acc_state_res_and_ready_updated_by_Acc_compute] >>
+  rw [Acc_compute_def] >-
+   (`(agp32 fext fbits (SUC t)).state = 2w` by gs [Abbr `s`,agp32_acc_arg_ready_then_next_state_2w] >>
+    gs [agp32_WB_state_flag_and_state]) >-
+   (Cases_on `t = 0` >-
+     (`~enable_stg 5 (agp32 fext fbits 0)` by fs [enable_stg_def,agp32_init_ctrl_flags] >>
+      `I' (5,SUC 0) = I' (5,0)` by fs [is_sch_def,is_sch_disable_def] >>
+      gs [is_sch_def,is_sch_init_def]) >>
+    `s'.acc_state = s.acc_state`
+      by METIS_TAC [Abbr `s`,Abbr `s'`,agp32_same_acc_items_until_Acc_compute] >>
+    `~s.acc_res_ready` by gs [agp32_acc_state_0w_then_acc_res_not_ready,Abbr `s`] >>
+    `s.state = 2w` by gs [agp32_acc_state_0w_then_state_2w,Abbr `s`] >>
+    `(agp32 fext fbits (SUC t)).state = (agp32_next_state (fext t) s s).state`
+      by fs [agp32_command_state_updated_by_agp32_next_state] >>
+    `(fext t).error = 0w` by fs [is_mem_def,mem_no_errors_def] >>
+    fs [agp32_next_state_def] >>
+    gs [agp32_WB_state_flag_and_state]) >-
+   (rw [acc_res_def,acc_arg_def,accelerator_f_def] >>
+    `I' (5,SUC t) = I' (5,t)` by fs [is_sch_def,is_sch_disable_def] >>
+    `(agp32 fext fbits t).WB.WB_opc = 8w` by fs [agp32_WB_opc_unchanged_when_WB_disabled] >>
+    fs [Rel_def,MEM_req_rel_def,Abbr `s`]) >>
+  `s'.acc_state = s.acc_state`
+    by METIS_TAC [Abbr `s`,Abbr `s'`,agp32_same_acc_items_until_Acc_compute] >>
+  METIS_TAC [agp32_acc_state_possible_values,Abbr `s`]
+QED
+
+
 (* MEM_data_rel *)
 Theorem agp32_Rel_ag32_MEM_data_rel_correct:
   !fext fbits a t I.
@@ -1344,7 +1389,8 @@ Theorem agp32_Rel_ag32_MEM_data_rel_correct:
 Proof
   rw [MEM_data_rel_def] >>
   METIS_TAC [agp32_Rel_ag32_read_mem_data_rdata_correct,
-             agp32_Rel_ag32_read_mem_byte_data_rdata_correct]
+             agp32_Rel_ag32_read_mem_byte_data_rdata_correct,
+             agp32_Rel_ag32_acc_res_correct]
 QED
 
 val _ = export_theory ();
